\documentclass{article}
\usepackage[utf8x]{inputenc}
\usepackage[T1, T2A]{fontenc}
\usepackage[russian]{babel}
\usepackage{amsmath}
\usepackage{amssymb}
\setlength\parindent{0pt}
\usepackage[parfill]{parskip}
\pagenumbering{gobble}

\begin{document}
Проще найти вероятность противоположного события:
\begin{align*}
1 - p(\triangle) &= p(Y \leqslant 1 - X) + p(Y \leqslant X-1) + p(Y \geqslant X+1)\\
&= \int\limits_0^1 \frac{t}{2} \frac{1-t}{3} dt + \int\limits_1^2 \frac{t}{2} \frac{t-1}{3} dt + \int\limits_0^2 \frac{t}{2} \frac{2-t}{3} dt\\
&= \frac{1}{36} + \frac{5}{36} + \frac{8}{36} = \frac{7}{18}.
\end{align*}
Тогда $$p(\triangle) = 1 - \frac{7}{18} = \frac{11}{18}.$$
\end{document}
