\documentclass{article}
\usepackage[utf8x]{inputenc}
\usepackage[T1, T2A]{fontenc}
\usepackage[russian]{babel}
\usepackage{amsmath}
\usepackage{amssymb}
\setlength\parindent{0pt}
\usepackage[parfill]{parskip}
\pagenumbering{gobble}
\usepackage{enumitem}

\begin{document}
$$\sum\limits_{k=0}^\infty (-1)^k \frac{(k+1)^2}{k!}=\sum\limits_{k=0}^\infty(-1)^k\frac{k^2}{k!}+\sum\limits_{k=0}^\infty (-1)^k\frac{2k}{k!}+\sum\limits_{k=0}^\infty(-1)^k \frac{1}{k!}=(*)$$

\begin{enumerate}[label=\alph*)]

\item

$$\sum\limits_{k=0}^\infty(-1)^k\frac{k^2}{k!}=\sum\limits_{k=1}^\infty(-1)^k\frac{k}{(k-1)!}=\sum\limits_{k=1}^\infty(-1)^k\frac{k-1+1}{(k-1)!}=$$
$$=\sum\limits_{k=2}^\infty(-1)^k\frac{1}{(k-2)!}+\sum\limits_{k=1}^\infty(-1)^k\frac{1}{(k-1)!}=$$
$$=(-1)^2\sum\limits_{l=0}^\infty(-1)^l\frac{1}{l!}+(-1)\sum\limits_{l=0}^\infty(-1)^l\frac{1}{l!}=0.$$

\item

$$\sum\limits_{k=0}^\infty (-1)^k\frac{2k}{k!}=2\sum\limits_{k=1}^\infty (-1)^k\frac{1}{(k-1)!}=-2\sum\limits_{l=0}^\infty (-1)^l\frac{1}{l!}=-\frac{2}{e}.$$

\end{enumerate}

$$(*)=-\frac{2}{e}+\frac{1}{e}=-\frac{1}{e}.$$
\end{document}
