\documentclass{article}
\usepackage[utf8x]{inputenc}
\usepackage[T1, T2A]{fontenc}
\usepackage[russian]{babel}
\usepackage{amsmath}
\usepackage{amssymb}
\setlength\parindent{0pt}
\usepackage[parfill]{parskip}
\pagenumbering{gobble}

\begin{document}
Сделаем замену $t=\sqrt{1 + e^x}$. Тогда
$$\int \frac{dx}{\sqrt{1+e^x}} = \int \frac{2 dt}{t^2 - 1} = \int \left( \frac{1}{t-1} - \frac{1}{t+1} \right) dt = \ln \frac{|t-1|}{|t+1|} + C.$$
Сделав обратную замену, получаем
$$\int \frac{dx}{\sqrt{1+e^x}} = \ln \frac{\sqrt{1+e^x} - 1}{\sqrt{1+e^x} + 1} + C.$$
\textit{Примечание.} Ответ можно также записать в виде
$$\int \frac{dx}{\sqrt{1+e^x}} = -2\, \textrm{arcth}\, (\sqrt{1+e^x}) + C,$$
где $\textrm{arcth}$ --- гиперболический арккотангенс.
\end{document}
