\documentclass{article}
\usepackage[utf8x]{inputenc}
\usepackage[T1, T2A]{fontenc}
\usepackage[russian]{babel}
\usepackage{amsmath}
\usepackage{amssymb}
\setlength\parindent{0pt}
\usepackage[parfill]{parskip}
\pagenumbering{gobble}

\begin{document}
Обозначим исходный интеграл через $I$. Произведем замену $x = \frac{1}{t}$.\\
Тогда
$$I = \int\limits_{\frac13}^3 \frac{\textrm{arctg}\, x}{x^2-x+1} dx = \int\limits_{\frac13}^3 \frac{\textrm{arcctg}\, t}{t^2 - t + 1} dt = $$
$$= \int\limits_{\frac13}^3 \frac{\frac{\pi}{2} - \textrm{arctg}\, t}{t^2 - t + 1} dt = \frac{\pi}{2} \int\limits_{\frac13}^3 \frac{dt}{t^2 - t + 1} dt - I.$$
Отсюда
$$I = \frac{\pi}{4} \int\limits_{\frac13}^3 \frac{dt}{t^2 - t + 1} dt = \frac{\pi}{2 \sqrt{3}} \textrm{arctg}\, \left. \left( \frac{2x-1}{\sqrt{3}} \right) \right|_{\frac13}^3 = $$
$$= \frac{\pi}{2\sqrt{3}} \left( \textrm{arctg}\, \frac{5}{\sqrt{3}} + \textrm{arctg}\, \frac{1}{3\sqrt{3}} \right) = \frac{\pi}{2\sqrt{3}} \textrm{arctg}\, 4\sqrt{3}.$$
\end{document}
