\documentclass{article}
\usepackage[utf8x]{inputenc}
\usepackage[T1, T2A]{fontenc}
\usepackage[russian]{babel}
\usepackage{amsmath}
\usepackage{amssymb}
\setlength\parindent{0pt}
\usepackage[parfill]{parskip}
\pagenumbering{gobble}

\begin{document}
Введем обозначение $b_n = \frac{1}{a_n}$. Тогда $b_{n+1} = \frac{1 + na_n}{a_n} = b_n + n$. Кроме того, $b_0 = \frac{1}{a_0} = 1$.\\
Получаем, что
$$b_n = b_0 + 1 + 2 + \cdots + n-1 = 1 + \frac{n(n-1)}{2} = \frac{n(n-1) + 2}{2}.$$
Отсюда получаем
$$a_n = \frac{2}{n(n-1)+2}.$$
\end{document}
